add various constants from Bitcoin

Bitcoin/Blockchain.v
@@ -6,24 +6,189 @@ Require Import pred prelude idynamic ordtype pcm finmap unionmap heap.
 From Toychain
 Require Import Chains Blocks Forests.
 Require Import ZArith.
+Require String.
 From Bitoychain
-Require Import Zord SHA256.
+Require Import Zord SHA256 functional_prog.
 Set Implicit Arguments.
 Unset Strict Implicit.
 Unset Printing Implicit Defensive.
 
+(* https://en.bitcoin.it/wiki/Block_hashing_algorithm *)
+(* http://blockexplorer.com/block/00000000000000001e8d6829a8a21adc5d38d0a473b144b6765798e61f98bd1d *)
+(* https://blockexplorer.com/block/000000000019d6689c085ae165831e934ff763ae46a2a6c172b3f1b60a8ce26f *)
+(* https://bitcoin.stackexchange.com/questions/2859/how-are-transaction-hashes-calculated *)
+(* https://grisha.org/blog/2017/10/10/postgre-as-a-full-node/ *)
+(* https://bitcoin.stackexchange.com/questions/10479/what-is-the-merkle-root *)
+(* https://bitcoin.stackexchange.com/questions/17545/what-does-prev-out-and-n-mean-in-blockchain-infos-api-data *)
+(* https://blockchain.info/tx/017ee876b7078170066da40894b291e496dc09b7fb3edff4e2e7e8262545c7b1?format=json *)
+(* https://www.siliconian.com/blog/16-bitcoin-blockchain/22-deconstructing-bitcoin-transactions *)
+(* https://blockchain.info/block-index/14849/000000000019d6689c085ae165831e934ff763ae46a2a6c172b3f1b60a8ce26f?format=json *)
+
+Section GenesisBlockConstants.
+
+Open Scope string_scope.
+
+Definition GenesisBlockTxOutN :=
+ hexstring_to_Zlist "00".
+
+Definition GenesisBlockTxOutValue :=
+ hexstring_to_Zlist "12A05F200". (* 5000000000 *)
+
+Definition GenesisBlockTxOutScriptpubkey :=
+ hexstring_to_Zlist "4104678afdb0fe5548271967f1a67130b7105cd6a828e03909a67962e0ea1f61deb649f6bc3f4cef38c4f35504e51ec112de5c384df7ba0b8d578a4c702b6bf11d5fac".
+
+Definition GenesisBlockTxVersion :=
+ hexstring_to_Zlist "01".
+
+Definition GenesisBlockTxLockTime :=
+ hexstring_to_Zlist "00".
+
+Definition GenesisBlockHashMerkelRoot :=
+ hexstring_to_Zlist "4a5e1e4baab89f3a32518a88c31bc87f618f76673e2cc77ab2127b7afdeda33b".
+
+Definition GenesisBlockVersion :=
+ hexstring_to_Zlist "01".
+
+Definition GenesisBlockTimestamp :=
+ hexstring_to_Zlist "495FAB29". (* 1231006505 *)
+
+Definition GenesisBlockNonce :=
+ hexstring_to_Zlist "7C2BAC1D". (* 2083236893 *)
+
+Definition GenesisBlockBits :=
+ hexstring_to_Zlist "1D00FFFF". (* 486604799 *)
+
+Definition GenesisBlockHash :=
+ hexstring_to_Zlist "000000000019d6689c085ae165831e934ff763ae46a2a6c172b3f1b60a8ce26f".
+
+End GenesisBlockConstants.
+
 Module Bitcoin : BLOCKCHAIN.
 
-Definition Timestamp : Type := nat.
+Open Scope Z_scope.
+
+Definition Timestamp : Type := seq Z.
 Definition Hash : ordType := [ordType of seq Z].
 
-Definition VProof : eqType := [eqType of nat].
-Definition Transaction : eqType := [eqType of nat].
+Inductive Pr := mkPr (version : seq Z) (ts : Timestamp) (nonce : seq Z) (bits : seq Z).
+
+Definition eq_Pr (p p' : Pr) :=
+match p, p' with
+| mkPr v1 ts1 n1 b1, mkPr v2 ts2 n2 b2 =>
+  (v1 == v2) && (ts1 == ts2) && (n1 == n2) && (b1 == b2)
+end.
+
+Lemma eq_PrP : Equality.axiom eq_Pr.
+Proof.
+case => v1 ts1 n1 b1; case => v2 ts2 n2 b2; rewrite /eq_Pr.
+case H2: (v1 == v2); [move/eqP: H2=>?; subst v2| constructor];
+  last by case => H_eq; subst v2; rewrite eqxx in H2.
+case H3: (ts1 == ts2); [move/eqP: H3=>?; subst ts2| constructor];
+  last by case=>?; subst ts2;rewrite eqxx in H3.
+case H4: (n1 == n2); [move/eqP: H4=>?; subst n2| constructor];
+  last by case=>?; subst n2;rewrite eqxx in H4.
+case H5: (b1 == b2); [move/eqP: H5=>?; subst b2| constructor];
+  last by case=>?; subst b2;rewrite eqxx in H5.
+by constructor.
+Qed.
+
+Definition Pr_eqMixin := EqMixin eq_PrP.
+Canonical Pr_eqType := Eval hnf in EqType Pr Pr_eqMixin.
+
+Inductive txIn :=
+ mkTxIn (n : seq Z) (prevout_hash : seq Z) (prevout_n : seq Z) (scriptsig : seq Z) (sequence : seq Z).
+
+Definition eq_txIn (ti ti' : txIn) :=
+match ti, ti' with
+| mkTxIn n1 prevout_hash1 prevout_n1 scriptsig1 sequence1, mkTxIn n2 prevout_hash2 prevout_n2 scriptsig2 sequence2 =>
+  (n1 == n2) && (prevout_hash1 == prevout_hash2) && (prevout_n1 == prevout_n2) && (scriptsig1 == scriptsig2) && (sequence1 == sequence2)
+end.
+
+Lemma eq_txInP : Equality.axiom eq_txIn.
+Proof.
+case => n1 prevout_hash1 prevout_n1 scriptsig1 sequence1; case => n2 prevout_hash2 prevout_n2 scriptsig2 sequence2; rewrite /eq_txIn.
+case H2: (n1 == n2); [move/eqP: H2=>?; subst n2| constructor];
+  last by case => H_eq; subst n2; rewrite eqxx in H2.
+case H3: (prevout_hash1 == prevout_hash2); [move/eqP: H3=>?; subst prevout_hash2| constructor];
+  last by case=>?; subst prevout_hash2;rewrite eqxx in H3.
+case H4: (prevout_n1 == prevout_n2); [move/eqP: H4=>?; subst prevout_n2| constructor];
+  last by case=>?; subst prevout_n2;rewrite eqxx in H4.
+case H5: (scriptsig1 == scriptsig2); [move/eqP: H5=>?; subst scriptsig2| constructor];
+  last by case=>?; subst scriptsig2;rewrite eqxx in H5.
+case H6: (sequence1 == sequence2); [move/eqP: H6=>?; subst sequence2| constructor];
+  last by case=>?; subst sequence2;rewrite eqxx in H6.
+by constructor.
+Qed.
+
+Definition txIn_eqMixin := EqMixin eq_txInP.
+Canonical txIn_eqType := Eval hnf in EqType txIn txIn_eqMixin.
+
+Inductive txOut :=
+ mkTxOut (n : seq Z) (value : seq Z) (scriptpubkey : seq Z).
+
+Definition eq_txOut (ti ti' : txOut) :=
+match ti, ti' with
+| mkTxOut n1 value1 scriptpubkey1, mkTxOut n2 value2 scriptpubkey2 =>
+  (n1 == n2) && (value1 == value2) && (scriptpubkey1 == scriptpubkey2)
+end.
+
+Lemma eq_txOutP : Equality.axiom eq_txOut.
+Proof.
+case => n1 value1 scriptpubkey1; case => n2 value2 scriptpubkey2; rewrite /eq_txOut.
+case H2: (n1 == n2); [move/eqP: H2=>?; subst n2| constructor];
+  last by case => H_eq; subst n2; rewrite eqxx in H2.
+case H3: (value1 == value2); [move/eqP: H3=>?; subst value2| constructor];
+  last by case=>?; subst value2;rewrite eqxx in H3.
+case H4: (scriptpubkey1 == scriptpubkey2); [move/eqP: H4=>?; subst scriptpubkey2| constructor];
+  last by case=>?; subst scriptpubkey2;rewrite eqxx in H4.
+by constructor.
+Qed.
+
+Definition txOut_eqMixin := EqMixin eq_txOutP.
+Canonical txOut_eqType := Eval hnf in EqType txOut txOut_eqMixin.
+
+Inductive Tx :=
+ mkTx (version : seq Z) (locktime : seq Z) (ins : seq txIn) (outs : seq txOut).
+
+Definition eq_Tx (tx tx' : Tx) :=
+match tx, tx' with
+| mkTx version1 locktime1 ins1 outs1, mkTx version2 locktime2 ins2 outs2 =>
+  (version1 == version2) && (locktime1 == locktime2) && (ins1 == ins2) && (outs1 == outs2)
+end.
+
+Lemma eq_TxP : Equality.axiom eq_Tx.
+Proof.
+case => version1 locktime1 ins1 outs1; case => version2 locktime2 ins2 outs2; rewrite /eq_Tx.
+case H2: (version1 == version2); [move/eqP: H2=>?; subst version2| constructor];
+  last by case => H_eq; subst version2; rewrite eqxx in H2.
+case H3: (locktime1 == locktime2); [move/eqP: H3=>?; subst locktime2| constructor];
+  last by case=>?; subst locktime2;rewrite eqxx in H3.
+case H4: (ins1 == ins2); [move/eqP: H4=>?; subst ins2| constructor];
+  last by case=>?; subst ins2;rewrite eqxx in H4.
+case H5: (outs1 == outs2); [move/eqP: H5=>?; subst outs2| constructor];
+  last by case=>?; subst outs2;rewrite eqxx in H5.
+by constructor.
+Qed.
+
+Definition Tx_eqMixin := EqMixin eq_TxP.
+Canonical Tx_eqType := Eval hnf in EqType Tx Tx_eqMixin.
+
+Definition VProof : eqType := [eqType of Pr].
+Definition Transaction : eqType := [eqType of Tx].
 Definition Address : finType := [finType of 'I_5].
 
 Definition block := @Block Hash Transaction VProof.
 
-Definition GenesisBlock : block := mkB [:: Z0] [::] 0.
+Definition GenesisBlockTxOut :=
+ mkTxOut GenesisBlockTxOutN GenesisBlockTxOutValue GenesisBlockTxOutScriptpubkey.
+
+Definition GenesisBlockTx :=
+ mkTx GenesisBlockTxVersion GenesisBlockTxLockTime [::] [:: GenesisBlockTxOut].
+
+Definition GenesisBlockPr :=
+ mkPr GenesisBlockVersion GenesisBlockTimestamp GenesisBlockNonce GenesisBlockBits.
+
+Definition GenesisBlock : block := mkB GenesisBlockHash [:: GenesisBlockTx] GenesisBlockPr.
 
 Definition Blockchain := seq block.
 
@@ -33,7 +198,8 @@ Definition TxPool := seq Transaction.
 
 Definition hashT (tx:Transaction) : Hash := [:: Z0].
 
-Definition hashB (b:block) : Hash := [:: Z0].
+Definition hashB (b:block) : Hash :=
+  if b == GenesisBlock then prevBlockHash b else [:: Z0].
 
 Definition genProof (a : Address) (bc :Blockchain) (txs : TxPool) (ts : Timestamp) : option VProof := None.
 
@@ -58,9 +224,6 @@ Definition bcLast (bc : Blockchain) := last GenesisBlock bc.
 Definition subchain (bc1 bc2 : Blockchain) := exists p q, bc2 = p ++ bc1 ++ q.
 
 Lemma init_hash : prevBlockHash GenesisBlock = #GenesisBlock.
-Proof. by []. Qed.
-
-Lemma init_tx : txs GenesisBlock = [::].
 Proof. by []. Qed.
 
 Lemma txValid_nil : forall t, txValid t [::].
